DecoupledConsensus.lean
@@ -1,3 +1,5 @@
 import DecoupledConsensus.AccountableSafety
+import DecoupledConsensus.State.Model
 import DecoupledConsensus.State
+import DecoupledConsensus.Store.Model
 import DecoupledConsensus.Store
